---
layout: post
title: "Differentiation"
author: "Karthik"
categories: journal
tags: [documentation,sample]
---


Sections: Integration of maps ${ f : [a, b] \to E }$; Mean value theorem

###### 4. 

$${ \underline{\textbf{Integration of maps } f : [a, b] \to E} }$$ 

Recall if a map is uniformly continuous and into a complete space, the domain of definition can be [expanded to its closure](https://math.stackexchange.com/a/4326834/303300) while preserving continuity of the map (and uniquely so). The extended map also turns out to be uniformly continuous. 

**Thm** [Extension of continuous linear maps]:    
Consider normed vector spaces ${ E }$ and ${ F, }$ with ${ E }$ complete. Let ${ F _0 \subseteq F }$ be a subspace, and ${ \lambda : F _0  \to E }$ a continuous linear map.    
Then ${ \lambda }$ has an extension ${ \overline{\lambda} : \overline{F _0} \to E }$ which is continuous linear. Also ${ \overline{\lambda}  }$ is the unique continuous map ${ \overline{F _0} \to E }$ which extends ${ \lambda ,  }$ and ${ \left\lVert \overline{\lambda} \right\rVert = \lVert \lambda \rVert }.$    

**Pf**: Firstly ${ \overline{F _0} }$ is also a vector subspace of ${ F :}$ Let ${ x, y \in \overline{F _0} }$ and ${ \alpha, \beta \in \mathbb{R} .}$ We are to show ${ \alpha x + \beta y \in \overline{F _0 } .}$ There are sequences ${ (x _n), (y _n) \subseteq F _0 }$ with ${ \lVert x _n - x \rVert \to 0, }$ ${ \lVert y _n - y \rVert \to 0 .}$ Now ${ \lVert (\alpha x _n + \beta y _n) - (\alpha x + \beta y) \rVert \to 0 }$ with sequence ${ (\alpha x _n + \beta y _n) \subseteq F _0 .}$ So ${ \alpha x + \beta y \in \overline{F _0 } .}$ 

Let ${ x \in \overline{F _0} .}$ (Equivalently, there is a sequence ${ (x _n) \subseteq F _0 }$ with ${ \lVert x _n - x \rVert \to 0 }$). If we show that    

* For any sequence ${ (x _n) \subseteq F _0 }$ with ${ \lVert x _n - x \rVert \to 0 ,}$ the limit ${ \lim _{n \to \infty} \lambda (x _n) }$ exists    
* For any two sequences ${ (x _n), (y _n) \subseteq F _0 }$ with ${ \lVert x _n - x \rVert \to 0, }$ ${ \lVert y _n - x \rVert \to 0 ,}$ the limits ${ \lim _{n \to \infty} \lambda(x _n) = \lim _{n \to \infty} \lambda(y _n) , }$ 

the natural extension map 

$${ \overline{\lambda} : \overline{F _0} \to E,  }$$ 

$${ \overline{\lambda}(x) := \left(\begin{align*} &\lim _{n \to \infty} \lambda(x _n), \text{ where } (x _n) \text{ is any sequence } \\  &\text{with } (x _n) \subseteq F _0 \text{ and }  \lVert x _n - x \rVert \to 0  \end{align*} \right) }$$ 

is well defined. 

These two properties are proved as in the previous result, so we have ${ \overline{\lambda} .}$ We are to show ${ \overline{\lambda} \in L(\overline{F _0}, E) .}$ 

Linearity of ${ \overline{\lambda} }$ is clear:    
Let ${ x , y \in \overline{F _0} .}$ There are sequences  ${ (x _n) , (y _n) \subseteq F _0 }$ with ${ \lVert x _n - x \rVert \to 0, }$ ${ \lVert y _n - y \rVert \to 0. }$ Now for any scalars ${ \alpha, \beta \in \mathbb{R}, }$ 

$${ \begin{align*} \overline{\lambda}(\alpha x + \beta y ) &= \lim _{n \to \infty} \lambda (\alpha x _n + \beta y _n) \quad (\text{as } \alpha x _n + \beta y _n  \to \alpha x + \beta y) \\ &= \lim _{n \to \infty} \alpha \lambda(x _n) + \beta \lambda (y _n) \\  &= \alpha \overline{\lambda}(x) + \beta \overline{\lambda}(y) . \end{align*} }$$ 

By the previous result, ${ \overline{\lambda} }$ is uniformly continuous. So ${ \overline{\lambda} \in L(\overline{F _0}, E) .}$ 

Uniqueness of the continuous extension ${ \overline{F _0} \to E }$ is clear. (Say ${ \lambda ^{’} : \overline{F _0} \to E }$ is another continuous extension of ${ \lambda .}$ Let ${ x \in \overline{F _0} .}$ There is a sequence ${ (x _n) \subseteq F _0 }$ with ${ \lVert x _n - x  \rVert \to 0 .}$ Now ${ \lambda ^{’} (x) }$ ${ = \lim _{n \to \infty} \lambda ^{’} (x _n) }$ ${ = \lim _{n \to \infty} \lambda  (x _n) }$ ${ = \overline{\lambda} (x) ,}$ as needed).

It is left to show that ${ \left\lVert \overline{\lambda} \right\rVert =  \lVert \lambda \rVert .  }$ Since 

$${ \left\lVert \overline{\lambda} \right\rVert = \sup _{v \in \overline{F _0}, v \neq 0} \frac{\left\lVert \overline{\lambda}(v) \right\rVert}{\lVert v \rVert} \geq \sup _{v \in F _0, v \neq 0} \frac{\left\lVert \overline{\lambda}(v) \right \rVert}{\lVert v \rVert} = \lVert \lambda \rVert  }$$

is clear, so we are to show ${ \left\lVert \overline{\lambda} \right\rVert \leq \lVert \lambda \rVert .}$ 

Let ${ v \in \overline{F _0 } .}$ There is a sequence ${ (x _n) \subseteq F _0 }$ with ${ \lVert x _n - v \rVert \to 0 .}$ As ${ \lVert \lambda (x _n) \rVert \leq \lVert \lambda \rVert \lVert x _n \rVert }$ and ${ \lim _{n \to \infty} \lambda(x _n) = \overline{\lambda}(v), }$ taking ${ n \to \infty }$ gives ${ \left\lVert \overline{\lambda}(v) \right\rVert }$ ${ \leq \lVert \lambda \rVert \lVert v \rVert .}$ So ${ \sup _{v \neq 0} \frac{\lVert \overline{\lambda} (v) \rVert}{\lVert v \rVert} \leq \lVert \lambda \rVert }$ that is ${ \left\lVert \overline{\lambda} \right\rVert \leq \lVert \lambda \rVert , }$ as needed. ${ \blacksquare }$ 

Consider reals ${ a < b , }$ and a complete normed space ${ E .}$ Recall the space of bounded functions ${ B([a, b], E) }$ with sup norm is [complete](https://bvenkatakarthik.github.io/UnifConv).    

We say ${ f : [a , b] \to E }$ is a step map if there is a partition ${ \mathcal{P} : a = x _0 < x _1 < \ldots < x _n = b }$ of ${ [a , b] }$ and elements ${ c _1, \ldots, c _n \in E }$ such that ${ f(t) = c _i }$ on each interval ${ (x _{i-1}, x _i) .}$ 

The set ${ \text{St}([a, b], E) }$ of step maps from ${ [a, b] }$ to ${ E }$ is a vector subspace of ${ B([a, b], E).  }$ The closure ${ \overline{\text{St}}([a , b], E) }$ is written as 

$${ \text{Reg}([a, b], E) := \overline{\text{St}}([a , b], E) ,}$$ 

and its elements are called regulated maps. 

**Thm** [Characterising regulated maps]:    

Consider reals ${ a < b }$ and a complete normed space ${ E .}$ Now the space of regulated maps 

$${ \text{Reg}([a, b], E) = \left\lbrace f \in B([a, b], E) \, : \,  \begin{align*} &\lim _{t \to x ^{+}} f(t) \text{ exists } \forall x \in [a, b), \\ &\lim _{t \to x ^{-}} f(t) \text{ exists } \forall x \in (a,b]   \end{align*} \right\rbrace . }$$ 

**Pf**: [Ref: Coleman’s book] 

${ \underline{\subseteq} }$: Let ${ f }$ be a regulated map. There is a sequence of step maps ${ (f _n) }$ converging to ${ f .}$ 

Let ${ x \in [a, b) .}$ We will show ${ \lim _{t \to x ^{+}} f(t) }$ exists. (A similar argument will show existence of left sided limits.) 

We are to show 

$${ \text{To show: } \lim _{t \to x ^{+}} f(t) \text{ exists} }$$

that is 

$${ \text{To show: } \quad \begin{align*} &\exists \ell \in E \text{ such that } \forall \text{ sequence } (t _n) \text{ in } (x, b] \\ &\text{with } \lim _{n \to \infty} t _n = x \text{ we have } \lim _{n \to \infty} f(t _n) = \ell  \end{align*} }$$ 

 that is 

$${ \begin{align*} &\text{To show: } \\ &{\color{red}{1)}} \, \forall \text{ sequence } (t _n) \text{ in } (x, b] \text{ converging to } x \text{ we have } \\ &\text{existence of } \lim _{n \to \infty} f(t _n)  \\ &{\color{blue}{2)}} \, \forall \text{ sequences } (s _n), (t _n) \text{ in } (x, b] \text{ converging to } x \text{ we have } \\ &\lim _{n \to \infty} f(s _n) = \lim _{n \to \infty} f(t _n) .  \end{align*} }$$ 

We will show a uniform-continuity-like condition 

$${ \text{Will show: } \quad \begin{align*} &\forall \varepsilon > 0 \, \exists \delta > 0 \text{ such that } \\ & p, q \in (x, x + \delta) \implies \lVert f(p) - f(q) \rVert < \varepsilon. \end{align*} }$$ 

Note that this guarantees both ${ 1) }$ and ${ 2) }$ above.    

For ${ {\color{red}{1)}} }$: Consider a sequence ${ (t _n) }$ in ${ (x, b] }$ with ${ \vert t _n - x \vert \to 0  .}$ We are to show sequence ${ (f(t _n)) }$ is Cauchy.    
Let ${ \varepsilon > 0 .}$ Pick a ${ \delta > 0 }$ such that ${ p, q \in (x, x + \delta) \implies \lVert f(p) - f(q) \rVert < \varepsilon. }$ Pick an ${ N }$ such that ${ n \geq N \implies t _n \in (x, x + \delta) .}$ Now 

$${ \begin{align*} m, n \geq N &\implies t _m, t _n \in (x, x + \delta) \\ &\implies \lVert f(t _m) - f(t _n) \rVert < \varepsilon, \end{align*} }$$

as needed. ${ {\color{red}{\blacksquare}} }$   
For ${ {\color{blue}{2)}} }$: Consider sequences ${ (s _n), (t _n) }$ in ${ (x, b] }$ with ${ \vert s _n - x \vert \to 0, }$ ${ \vert t _n - x \vert \to 0 .}$ By ${ 1) , }$ say ${ \lim _{n \to \infty} f(s _n) = \ell _s }$ and ${ \lim _{n \to \infty} f(t _n) = \ell _t .}$ We are to show ${  \ell _s = \ell _t .}$ Since  

$${ \begin{align*} &\lVert \ell _s - \ell _t  \rVert \\ \leq \, &\underbrace{\lVert \ell _s  - f(s _n) \rVert} _{\to 0} + \lVert f(s _n) - f(t _n) \rVert + \underbrace{\lVert f(t _n) - \ell _t  \rVert} _{\to 0},  \end{align*} }$$ 

it suffices to show ${ \lVert f(s _n) - f(t _n) \rVert \to 0 .}$    
Let ${ \varepsilon > 0 .}$ Pick a ${ \delta > 0 }$ such that ${ p, q \in (x, x + \delta) \implies \lVert f(p) - f(q) \rVert < \varepsilon. }$ Pick an ${ N }$ such that ${ n \geq N \implies s _n, t _n \in (x, x + \delta) .}$ Now 

$${ \begin{align*} n \geq N &\implies s _n, t _n \in (x, x + \delta) \\ &\implies \lVert f(s _n) - f(t _n) \rVert < \varepsilon, \end{align*}  }$$ 

as needed. ${ {\color{blue}{\blacksquare}} }$ 

We will show the uniform-continuity-like condition used for proving ${ {\color{red}{1)}} }$ and ${ {\color{blue}{2)}} .}$ 

$${ \text{To show: } \quad \begin{align*} &\forall \varepsilon > 0 \, \exists \delta > 0 \text{ such that } \\ & p, q \in (x, x + \delta) \implies \lVert f(p) - f(q) \rVert < \varepsilon. \end{align*} }$$ 

Let ${ \varepsilon > 0 .}$ There is an ${ N }$ such that ${ \lVert f _N - f \rVert < \varepsilon .}$ As ${ f _N }$ is a step map, there is a ${ \delta > 0 }$ such that ${ f _N }$ is constant over ${ (x, x + \delta) .}$ Now for ${ p, q \in (x, x + \delta) , }$ 

$${ \begin{align*} &\lVert f(p) - f(q) \rVert \\ \leq \, &\underbrace{\lVert f(p) - f _N (p) \rVert} _{ < \varepsilon \text{ as } \lVert f _N - f \rVert < \varepsilon}  +  \underbrace{\cancel{\lVert f _N (p) - f _N (q) \rVert}} _{f _N \text{ constant over } (x , x + \delta) } + \underbrace{\lVert f _N (q) - f (q) \rVert} _{< \varepsilon \text{ as } \lVert f _N - f \rVert < \varepsilon} \\ < \, &2\varepsilon,     \end{align*} }$$ 

as needed. 

${ \underline{\supseteq} }$: Say ${ f \in B([a, b], E) }$ satisfies the left and right limit criteria. Let ${ \varepsilon > 0 .}$ We are to show there is a step map ${ \phi }$ with ${ \lVert f - \phi \rVert < \varepsilon .}$ 

It suffices to show 

$${ \text{To show: } \quad \begin{align*} &\exists \text{ a partition } \mathcal{P} = (y _i) \text{ of } [a, b] \text{ such that } \\ &p, q  \in (y _{i-1}, y _i) \implies \lVert f(p) - f(q) \rVert < \varepsilon,  \end{align*} }$$ 

because then for example the map ${ \phi }$ where 

$${ \phi (t) = \begin{cases} f\left( \frac{y _{i-1} + y _i}{2} \right) &\text{ for } t \in (y _{i-1}, y _i) \\ f(t)  &\text{ for } t \in \mathcal{P} \end{cases}   }$$

works. 

For each ${ x \in [a, b), }$ as ${ \lim _{t \to x ^{+} } f(t) }$ exists, there is a ${ \delta _x > 0 }$ such that 

$${ p, q \in (x, x + \delta _x) \implies \lVert f(p) - f(q) \rVert < \varepsilon. }$$

For each ${ x \in (a, b], }$ as ${ \lim _{t \to x ^{-}} f(t) }$ exists, there is a ${ \Delta _x > 0 }$ such that 

$${ p, q \in (x - \Delta _x, x) \implies \lVert f(p) - f(q) \rVert < \varepsilon . }$$ 

These give an open cover 

$${ [a, b] =  [a, a + \delta _a) \cup (b - \Delta _b, b] \cup  \bigcup _{x \in (a, b)} (x - \Delta _x, x + \delta _x).   }$$ 

The sets ${ [a, a + \delta _a) }$ and ${ (b - \Delta _b, b] }$ are open in the space ${ [a, b] .}$

As ${ [a, b] }$ is compact, the above open cover has a finite subcover. The finite subcover must have ${ [a, a + \delta _a) }$ and ${ (b - \Delta _b, b] }$: They are the only sets of the cover containing ${ a }$ and ${ b }$ respectively. 

So there is a finite subcover 
$${ [a, b] = [a, a + \delta _a) \cup (b - \Delta _b, b] \cup \bigcup _{i=1} ^{n} (x _i - \Delta _{x _i}, x _i +  \delta _{x _i})  }$$ 

with ${ x _1, \ldots, x _n \in (a, b) .}$ 

 Taking ${ \mathcal{P} }$ to be the partition produced by ordering the points 

 $${ \lbrace a , a + \delta _a; b - \Delta _b, b; x _1 - \Delta _{x _1}, x _1, x _1 + \delta _{x _1} ; \ldots; x _n - \Delta _{x _n}, x _n, x _n + \delta _{x _n}  \rbrace  }$$ 

 works: Say ${ \mathcal{P} = (y _i). }$ Now each interval ${ (y _{i-1}, y _{i}) }$ is contained in a set of the form ${ (x - \Delta _x, x) }$ or ${ (x, x + \delta _x)  }$ and hence satisfies 

 $${ p, q \in (y _{i-1}, y _i) \implies \lVert f(p) - f(q) \rVert < \varepsilon, }$$

as needed. ${ \blacksquare }$ 

A map ${ f : [a, b] \to E }$ is piecewise continuous if there is a partition ${ \mathcal{P} : a = x _0 < x _1 < \ldots < x _n = b }$ such that for each ${ i }$ the restriction ${ f   : (x _{i-1}, x _i) \to E }$ admits a continuous extension ${ f _i : [x _{i-1}, x _i] \to E .}$ 

By the above result, piecewise continuous maps ${ [a, b] \to E }$ into a complete space are regulated. 

We can now consider integrating step maps (This, along with linear extension theorem, will allow us to integrate regulated maps). 

**Def** [Integral of a step map wrt a partition]:    
Consider reals ${ a < b, }$ a complete normed space ${ E }$ and a step map ${ f : [a, b] \to E .}$    
Say ${ \mathcal{P} : a = x _0 < \ldots < x _n = b }$ is a partition wrt which ${ f }$ is a step map, and ${ f(t) = c _i }$ on each interval ${ t \in (x _{i-1}, x _i) .}$ Then the integral of ${ f }$ wrt ${ \mathcal{P} }$ is defined as 

$${ I _{\mathcal{P}} (f) := \sum _{i=1} ^n c _i (x _i - x _{i-1}) .  }$$ 

**Obs**: Consider reals ${ a < b, }$ a complete normed space ${ E }$ and a step map ${ f : [a, b] \to E .}$    
Say ${ f }$ is a step map wrt partition ${ \mathcal{P} : a = x _0 < \ldots < x _n = b ,}$ and ${ \hat{x} \in (a, b) .}$    
Then ${ f }$ is a step map wrt the partition described by points ${ \mathcal{P} \cup \lbrace \hat{x} \rbrace,  }$ and 

$${ I _{\mathcal{P} \cup \lbrace \hat{x} \rbrace} (f) = I _{\mathcal{P}} (f). }$$    

**Pf**: If ${ \hat{x} }$ is some ${ x _j  }$ then ${ \mathcal{P} \cup \lbrace \hat{x} \rbrace = \mathcal{P} }$ and we are done, so say ${ \hat{x} }$ lies in some ${ (x _{j-1}, x _j) .}$    
Say ${ f(t) = c _i }$ on each interval ${ t \in (x _{i-1}, x _i ) .}$ We see ${ f }$ is a step map wrt partition ${ \mathcal{P} \cup \lbrace \hat{x} \rbrace,  }$ and 

$${ \begin{align*} I _{\mathcal{P} \cup \lbrace \hat{x} \rbrace } (f) = &\sum _{i < j} c _i (x _i - x _{i-1}) + c _{j} (\hat{x} - x _{j-1}) + c _j (x _j - \hat{x}) \\ &\, + \sum _{i > j}  c _i (x _i - x _{i-1}) \\ = &\sum _{i} c _i (x _{i+1} - x _i) \\ = &I _{\mathcal{P}} (f)  \end{align*} }$$ 

as needed. 

**Obs**: Consider reals ${ a < b, }$ a complete normed space ${ E }$ and a step map ${ f : [a, b] \to E .}$    
If ${ f }$ is a step map wrt both partitions ${ \mathcal{P} }$ and ${ \mathcal{Q}, }$ then

$${ I _{\mathcal{P}} (f) = I _{\mathcal{Q}} (f) .}$$ 

**Pf**: Adding finitely many points to a partition ensures ${ f }$ is still a step map wrt new partition and integral of ${ f }$ wrt new partition is same as the old one.    
So ${ f }$ is a step map wrt partition described by points ${ \mathcal{P} \cup \mathcal{Q}, }$ and 

$${ I _{\mathcal{P}} (f) = I _{\mathcal{P} \cup \mathcal{Q}} (f) = I _{\mathcal{Q}} (
f) }$$ 

as needed. 

**Def** [Integral of a step map]:    
Consider reals ${ a < b, }$ a complete normed space ${ E }$ and a step map ${ f : [a, b] \to E .}$    
By the above observation, we can define the integral of ${ f }$ as 

$${ I(f) := I _{\mathcal{P}} (f) ,}$$ 

where ${ \mathcal{P} }$ is any partition wrt which ${ f }$ is a step map.   

**Obs** [Linearity of integral for step maps]:    
Consider reals ${ a < b }$ and a complete normed space ${ E .}$ The integration operation on step maps 

$${ I : \text{St}([a, b], E) \longrightarrow E }$$ 

is continuous linear with ${ \lVert I(f) \rVert \leq (b-a) \lVert f \rVert. }$ 

**Pf**: Say ${ f , g : [a, b] \to E }$ are step maps wrt partitions ${ \mathcal{P} _f, \mathcal{P} _g }$ respectively, and ${ \alpha, \beta \in \mathbb{R} .}$    
Now ${ \alpha f + \beta g , f, g }$ are step maps wrt the partition described by points ${ \mathcal{P} _f \cup \mathcal{P} _g .}$ Say the partition described by points ${ \mathcal{P} _f \cup \mathcal{P} _g }$ is ${ a = x _0 < \ldots < x _n = b , }$ and ${ f(t) = c _i, g(t) = d _i }$ on each interval ${ t \in (x _{i-1}, x _i) .}$ This gives 

$${ \begin{align*} I(\alpha f + \beta g) = &\sum _{i=1} ^{n} (\alpha c _i + \beta d _i) (x _{i} - x _{i-1}) \\ = &\alpha \sum _{i=1} ^{n} c _i (x _i - x _{i-1}) + \beta \sum _{i=1} ^{n} d _i (x _i - x _{i-1}) \\ =  &\alpha I(f) + \beta I(g), \end{align*} }$$ 

so ${ I }$ is linear. Further 

$${ \begin{align*} \lVert I(f) \rVert \leq &\sum _{i=1} ^{n} \lVert c _i \rVert  (x _i - x _{i-1}) \\ \leq &\, \lVert f \rVert \sum _{i=1} ^{n} (x _i - x _{i-1}) \\ = &\, \lVert f \rVert (b-a)  ,  \end{align*} }$$ 

so especially ${ I }$ is continuous. ${ \blacksquare }$ 

Consider reals ${ a < b }$ and a complete normed space ${ E .}$ By linear extension theorem, we can extend the above map to a continuous linear map 

$${ I : \overline{\text{St}}([a, b], E)  \longrightarrow E,  }$$ 

$${ I(f) := \left( \begin{align*} &\lim _{n \to \infty} I(f _n), \text{ where } (f _n) \text{ is any sequence} \\  &\text{in } \text{St}([a, b], E) \text{ with }  \lVert f _n - f \rVert \to 0  \end{align*} \right) . }$$ 

We write ${ I(f) }$ as 

$${ I(f) = \int _{a} ^{b} f .}$$ 

**Obs**: Consider reals ${ a < b ,}$ a complete normed space ${ E }$ and a step map ${ f : [a, b] \to E .}$    
If ${ c \in [a, b], }$ then both ${ f \vert _{[a, c]} }$ and ${ f \vert _{[c, b]} }$ are step maps and 

$${ I(f \vert _{[a, b]}) = I(f \vert _{[a, c]}) + I(f \vert _{[c, b]}) . }$$    

**Pf**: Say ${ f : [a, b] \to E }$ is a step map wrt partition ${ \mathcal{P} : a = x _0 < \ldots < x _n = b ,}$ and ${ c \in [a, b] .}$ If ${ c }$ is some ${ x _j }$ the result is clear, so say ${ c }$ lies in some ${ (x _{j-1}, x _j) .}$ 

Say ${ f(t) = c _i }$ on each interval ${ t \in (x _{i-1}, x _i) .}$ We see ${ f \vert _{[a, b]}, f \vert _{[a, c]} , f \vert _{[c, b]} }$ are step maps wrt partition ${ \mathcal{P} \cup \lbrace c \rbrace }$ restricted to ${ [a, b], [a, c], [c, b] }$ respectively. Also 

$${ \begin{align*} I(f \vert _{[a, b]}) = &\sum _{i=1} ^{n} c _i (x _i - x _{i-1}) \\ = &\sum _{i < j} c _i (x _i - x _{i-1}) +  c _j (c - x _{j-1}) \\ &+ c _j (x _j - c) + \sum _{i > j} c _i (x _i - x _{i-1}) \\ = &I(f \vert _{[a, c]}) + I(f \vert _{[c, b]}) \end{align*} }$$ 

as needed. 

**Obs** [Monotonicity of integral for step maps]:    
Consider reals ${ a < b , }$ and step maps ${ f, g : [a, b] \to \mathbb{R} .}$ Then 

$${ f \leq g \implies I(f) \leq I(g). }$$ 

**Pf**: Say ${ f, g : [a, b] \to \mathbb{R} }$ are step maps wrt partitions ${ \mathcal{P} _f, \mathcal{P} _g }$ respectively. Now both ${ f, g }$ are step maps wrt the partition defined by points ${ \mathcal{P} _f \cup \mathcal{P} _g .}$ Say the partition described by points ${ \mathcal{P} _f \cup \mathcal{P} _g }$ is ${ a = x _0 < \ldots < x _n = b , }$ and ${ f(t) = c _i, g(t) = d _i }$ on each interval ${ t \in (x _{i-1}, x _i) .}$

Let ${ f \leq g . }$ So each ${ c _i \leq d _i .}$ Then 

$${ \begin{align*} I(f) = &\sum _{i=1} ^{n} c _i (x _i - x _{i-1}) \\ \leq &\sum _{i=1} ^{n} d _i (x _i - x _{i-1}) \\ = &\, I(g) ,  \end{align*} }$$ 

as needed. 

**Def**: Consider reals ${ \alpha < \beta , }$ a complete normed space ${ E }$ and a regulated map ${ f : [\alpha, \beta] \to E .}$    
For ${ a \leq b }$ in ${ [\alpha, \beta],  }$  note ${ f \vert _{[a, b]} }$ is regulated too. (If step maps ${ f _n }$ are uniformly convergent to ${ f ,}$ the step maps ${ f _n \vert _{[a, b]} }$ are uniformly convergent to ${ f \vert _{[a, b]} }$). We define 

$${ \int _{b} ^{a} f := - \int _{a} ^{b} f . }$$  

**Thm**: Consider reals ${ \alpha < \beta , }$ a complete normed space ${ E }$ and a regulated map ${ f : [\alpha, \beta] \to E .}$    
Then for ${a, b, c \in [\alpha, \beta], }$ 

$${ \int _{a} ^{b} f = \int _{a} ^{c} f +  \int _{c} ^{b} f . }$$ 

**Pf**:  As ${ f }$ is regulated, there are step maps ${ f _n : [\alpha, \beta] \to E }$ uniformly converging to ${ f : [\alpha, \beta] \to E .}$ 

Consider first the case ${ a \leq c \leq b .}$ So step maps ${ f _n \vert _{[a, b]}, }$ ${ f _n \vert _{[a, c]}, }$ ${ f _n \vert _{[c, b]}   }$ are uniformly convergent to ${ f \vert _{[a, b]} , }$ ${ f \vert _{[a, c]} , }$ ${ f \vert _{[c, b]} }$ respectively. We are to show ${ \int _{a} ^{b} f = \int _{a} ^{c} f + \int _{c} ^{b} f }$ that is ${ \lim I(f _n \vert _{[a, b]}) =  \lim I(f _n \vert _{[a, c]}) + \lim I(f _n \vert _{[c, b]}),  }$ which is true. 

Consider the case ${ a \leq b \leq c .}$ We are to show ${ \int _{a} ^{b} f = \int _{a} ^{c} f + \int _{c} ^{b} f }$ that is ${ \lim I(f _n \vert _{[a, b]}) = \lim I(f _n \vert _{[a, c]}) + (-\lim I(f _n \vert _{[b, c]}) ),  }$ which is true. 

One can verify the truth of ${ \int _{a} ^{b} f = \int _{a} ^{c} f + \int _{c} ^{b} f }$ for the remaining ${ 3! - 2 = 4 }$ orderings of ${ a, b, c \in [\alpha, \beta] }$ similarly. 

**Thm** [Monotonicity of integral]:    
Consider reals ${ a < b , }$ and regulated maps ${ f, g : [a, b] \to \mathbb{R} .}$ Now 

$${ f \leq g \implies \int _{a} ^{b} f  \leq \int _{a} ^{b} g .  }$$ 

**Pf**: As ${ f, g }$ are regulated, so is ${ g - f .}$ The proof of characterisation of ${ \text{Reg}([a, b], E) }$ gives, for every ${ \varepsilon > 0 }$ a specific step map ${ \phi _{\varepsilon} }$ such that ${ \lVert (g - f) - \phi _{\varepsilon} \rVert < \varepsilon .}$ 

Let ${ g - f \geq 0 . }$ With this, the considered step maps ${ \phi _{\varepsilon} }$ are also ${ \geq 0 .}$    

So the step maps ${ \phi _{\frac{1}{n}} }$ are ${ \geq 0 }$ and uniformly convergent to ${ g - f ,}$ giving 

$${ \int _{a} ^{b} (g-f) = \lim _{n \to \infty} I\left(\phi _{\frac{1}{n}}\right) \geq 0   }$$ 

as needed. 

**Obs** [Uniform limit and Integral]:    
Consider reals ${ a < b, }$ a complete normed space ${ E ,}$ and a sequence of regulated maps ${ f _n : [a, b] \to E }$ with ${ \lVert f _n - f \rVert \to 0 }$ for some ${ f : [a, b] \to E .}$    
Uniform limit of bounded maps [is bounded](https://bvenkatakarthik.github.io/UnifConv), so ${ f }$ is in ${ B([a, b], E) .}$ As ${ \text{Reg}([a, b], E) }$ is closed in ${ B([a, b], E), }$ the limit ${ f  }$ is in ${ \text{Reg}([a, b], E) . }$ As 

$${ \int _a ^b  : \text{Reg}([a, b] , E) \longrightarrow E  }$$ 

is continuous linear, 

$${ \int _a ^b f _n \longrightarrow \int _{a} ^{b} f .  }$$ 

So uniform limit of regulated maps is regulated, and here integral of limit is limit of integrals. 

**Thm** [Bound for integral]:    
Consider reals ${ \alpha < \beta , }$ a complete normed space ${ E }$ and a regulated map ${ f : [\alpha, \beta] \to E . }$    
Then for ${ x, c \in [\alpha, \beta], }$ 

$${ \left\lVert \int _{c} ^{x} f \right\rVert \leq \vert x - c \vert \lVert f \rVert .  }$$ 

For ${ c \in [\alpha, \beta] ,}$ the map ${ F: [\alpha, \beta] \to E , }$ ${ F(t) =  \int _{c} ^{t} f }$ is uniformly continuous. 

**Pf**: As ${ f }$ is regulated, there is a sequence of step maps ${ f _n : [\alpha, \beta] \to E }$ uniformly converging to ${ f : [\alpha, \beta] \to E .}$    
**i**) It suffices to show the inequality for ${ c \leq x }$ case. Note step maps ${ f _n \vert _{[c, x]} }$ uniformly converge to ${ f \vert _{[c, x]} .}$ Each step map ${ f _n \vert _{[c, x]} }$ satisfies 

$${ \begin{align*}  \lVert I(f _n \vert _{[c, x]}) \rVert \leq &(x-c) \lVert f _n \vert _{[c, x]} \rVert \\ \leq &(x - c) \lVert f _n \rVert,  \end{align*} }$$ 

so limit ${ n \to \infty }$ gives 

$${ \left\lVert \int _{c} ^{x} f \right\rVert \leq  (x - c) \lVert f \rVert  }$$ 

as needed.    
**ii**) The map ${ F: [\alpha, \beta] \to E , }$ ${ F(t) =  \int _{c} ^{t} f }$ is uniformly continuous because for all ${ x, y \in [\alpha, \beta], }$ 

$${  \lVert F(x) - F(y) \rVert = \left\lVert \int _{y} ^{x} f \right\rVert \leq \vert x - y \vert \lVert f \rVert .  }$$ 

**Thm**: A map ${ f : [a, b] \to \mathbb{R} ^k , }$ ${ f = (f _1, \ldots, f _k) ^T }$ is regulated if and only if each ${ f _i }$ is regulated. In this case, 

$${ \int _a ^b f = \left( \int _a ^b f _1, \ldots, \int _a ^b f _k  \right) .}$$ 

**Pf**: ${ \underline{\Rightarrow} }$ Say ${ f : [a, b] \to \mathbb{R} ^k , }$ ${ f = (f _1, \ldots, f _k) ^T }$ is regulated. So there are step maps ${ s _n : [a, b] \to \mathbb{R} ^k, }$ ${ s _n  = ((s _n) _1, \ldots, (s _n) _k) ^T }$ with ${ \lVert s _n - f \rVert \to 0 .}$    
Now for each ${ i = 1, \ldots, k, }$ 

$${ \begin{align*} \lVert (s _n ) _i - f _i \rVert = &\sup _{x \in [a, b]}  \vert (s _n) _i (x) - f _i (x) \vert \\ \leq &\sup _{x \in [a, b]} \sqrt{\sum _{j=1} ^{k} \vert (s _n) _j (x) - f _j (x) \vert ^2} \\ = &\lVert s _n - f \rVert \to 0 \end{align*}  }$$ 

with ${ (s _n) _i  }$ step maps. Especially each ${ f _i }$ is regulated.   

Note if ${ s _n : [a, b] \to \mathbb{R} ^k }$ is step map wrt partition ${ \mathcal{P} _n ,}$ then ${ (s _n) _1, \ldots, (s _n) _k : [a, b] \to \mathbb{R}  }$ are step maps wrt same partition, and 

$${ I _{\mathcal{P} _n} (s _n) = \left( I _{\mathcal{P} _n} ((s _n) _1), \ldots, I _{\mathcal{P} _n} ((s _n) _k ) \right) }$$ 

that is 

$${ I  (s _n) = \left( I ((s _n) _1), \ldots, I ((s _n) _k ) \right) .  }$$ 

Since ${ \lVert s _n - f \rVert \to 0 }$ and each ${ \lVert (s _n) _i - f _i \rVert \to 0, }$ taking ${ n \to \infty }$ gives 

$${   \int _a ^b f = \left( \int _a ^b f _1, \ldots, \int _a ^b f _k  \right) .}$$ 

${ \underline{\Leftarrow} }$: Say ${ f : [a, b] \to \mathbb{R} ^k , }$ ${ f = (f _1, \ldots, f _k) ^T }$ is such that each ${ f _i }$ is regulated. We are to show ${ f }$ is regulated.    
For each ${ f _i }$ there are step maps ${ (s _i) _n : [a, b] \to \mathbb{R} }$ with ${ \lVert (s _i) _n - f _i \rVert \to 0 .}$    
If ${ (s _1) _n, \ldots, (s _k) _n : [a, b] \to \mathbb{R} }$ are step maps wrt partitions ${ \mathcal{P} _{1, n}, \ldots, \mathcal{P} _{k,n} }$ then 

$${ S _n := ((s _1) _n, \ldots, (s _k) _n) }$$

is a step map wrt partition described by points ${ \mathcal{P} _n := \mathcal{P} _{1, n} \cup \ldots \cup \mathcal{P} _{k, n} .}$ Further, 

$${ \begin{align*} \lVert S _n - f \rVert = &\sup _{x \in [a, b]} \sqrt{\sum _{i=1} ^{k} [(s _i) _n (x) - f _i (x)] ^2  } \\ \leq &\sqrt{\sum _{i=1} ^{k} \lVert (s _i) _n (x) - f _i \rVert ^2 } \to 0 \end{align*}   }$$ 

so ${ f }$ is regulated, as needed. 

**Thm** [Integral as antiderivative]:    
Consider reals ${ a < b ,}$ a complete normed space ${ E }$ and a regulated map ${ f : [a, b] \to E .}$ Let 

$${ F : [a, b] \to E, \quad F(x) := \int _a ^x f .}$$ 

If ${ f }$ is continuous at ${ c \in [a, b] , }$ then 

$${  F ^{’} (c) = f(c) . }$$ 

> For ${ E = \mathbb{R} }$ it is intuitively clear: Area ${ F(c + h) \approx F(c) + f(c) h . }$ 

**Pf**: Say ${ f }$ is continuous at ${ c \in [a, b] .}$    
For ${ h }$ such that ${ h \neq 0, }$ ${ c + h \in [a, b] }$ we have 

$${ \begin{align*} \frac{F(c+h) - F(c)}{h} - f(c) = &\frac{1}{h} \left(\int _{c} ^{c+h} f \right) - f(c) \\ = &\frac{1}{h} \int _{c} ^{c+h} (f - f(c)).   \end{align*} }$$ 

Let ${ \varepsilon > 0 .}$ By continuity at ${ c,}$ there is a ${ \delta > 0 }$ such that 

$${ x \in [a, b], \,  \vert x - c \vert < \delta \implies \lVert f(x) - f(c) \rVert < \varepsilon .}$$ 

Recall segment notation ${ [[ \alpha, \beta ]] := \lbrace \alpha + t(\beta - \alpha) : t \in [0, 1] \rbrace .}$ Now 

$${ \begin{align*} \left\lVert  \frac{F(c+h) - F(c)}{h} - f(c) \right\rVert = &\, \frac{1}{\vert h \vert}  \left\lVert \int _{c} ^{c+h} (f - f(c)) \right\rVert \\ \leq &\sup _{x \in [[c, c+h]]} \lVert f(x) - f(c) \rVert \\ {\color{blue}{\leq}} &\, \varepsilon \end{align*} }$$ 

for ${ h }$ such that ${ h \neq 0, }$ ${ c + h \in [a, b] }$ and ${ {\color{blue}{\vert h \vert < \delta}} . }$ So 

$${ \frac{F(c+h) - F(c)}{h} \longrightarrow f(c) }$$ 

as ${ c + h \in [a, b], }$ ${ h \to 0 .}$ ${ \blacksquare }$ 

**Thm** [Integral as the only antiderivative, upto constants]:    
Consider reals ${ a < b ,}$ a complete normed space ${ E }$ and a continuous map ${ f : [a, b] \to E .}$ Let 

$${ F : [a, b] \to E, \quad F(x) := \int _a ^x f .}$$  

By the above observations, ${ F : [a, b] \to E }$ is a continuous antiderivative of ${ f , }$ that is 

$${ \left\lbrace \begin{align*} &F \text{ is continuous on } [a, b]; \\  &D F  (x) = f(x) \text{ for all } x \in (a, b) \end{align*} \right\rbrace .}$$ 

Say ${ \hat{F} : [a, b] \to E }$ is another continuous antiderivative of ${ f . }$ Then ${ F, \hat{F} : [a, b] \to E }$ differ by a constant. 

> So ${ \int _{a} ^{x} f = \hat{F}(x) + c   ,}$ and setting ${ x =  a }$ gives 
> 
> $${ \int _{a} ^{x} f = \hat{F}(x) - \hat{F}(a) .}$$ 
> 
> Especially 
> 
> $${ \int _a ^b f = \hat{F}(b) - \hat{F}(a). }$$ 

**Pf**: We have ${ D (F - \hat{F})  (x) = 0 }$ for all ${ x \in (a, b) .}$ By the lemma below, ${ F - \hat{F} }$ is constant on ${ (a, b) .}$  But ${ F - \hat{F} }$ is continuous on ${ [a, b], }$ so it is constant on ${ [a, b] .  }$ 

**Lem**: Consider reals ${ a < b , }$ a complete normed space ${ E }$ and a map ${ f : [a, b] \to E .}$    
If ${ Df(t) = 0 }$ for all ${ t \in (a, b) , }$ then ${ f }$ is constant on ${ (a, b) .}$    

**Pf**: Consider points ${ \alpha < \beta }$ in ${ (a, b) .}$ We will show ${ f(\alpha) = f(\beta) .}$    

Let ${ \varepsilon > 0 .}$ For every ${ t \in [\alpha, \beta] }$ there is a ${ \delta _t > 0 }$ such that 

$${ \vert h \vert  < \delta _t \implies \lVert f(t + h) - f(t) - \cancel{Df(t) h} \rVert  \leq \varepsilon \vert h \vert }$$ 

that is 

$${ x \in (t - \delta _t, t + \delta _t)  \implies \lVert f(x) - f(t) \rVert \leq \varepsilon \vert x - t \vert .}$$ 

This is local information for every ${ t \in [\alpha, \beta], }$ but compactness lets us work with it. 

Consider the open cover 

$${ [\alpha, \beta] \subseteq \bigcup _{t \in [\alpha, \beta]} (t - \delta _t, t + \delta _t).  }$$ 

By compactness of ${ [\alpha, \beta] , }$ it has a finite subcover 

$${ [\alpha, \beta] \subseteq \bigcup _{i=1} ^{n} (t _i - \delta _{t _i}, t _i + \delta _{t _i})  .}$$ 

WLOG no element of the cover is contained in another element of the cover (because if so, the element contained can be removed). Order the centers ${ t _i }$ so that 

$${ \alpha \leq t _1 < \ldots < t _n \leq \beta .}$$ 
 
Note if some ${ (t _i - \delta _i, t _i + \delta _i) }$ and ${ (t _{i+1} -  \delta _{i+1}, t _{i+1} + \delta _{i+1}) }$ do not intersect, that is ${ t _i + \delta _i <  t _{i+1} -  \delta _{i+1} , }$ then the segment ${ [ t _i + \delta _i, t _{i+1} -  \delta _{i+1}  ] }$ doesnt intersect any of ${ (t _1 - \delta _1, t _1 + \delta _1), \ldots, (t _n - \delta _n, t _n + \delta _n) , }$ a contradiction. 

So for each ${ i = 1, \ldots, n -1  }$ we can pick an ${ {\color{blue}{x _i}}  \in (t _{i}, t _{i+1}) }$ in the intersection of ${ (t _i - \delta _i, t _i + \delta _i) }$ and ${ (t _{i+1} -  \delta _{i+1}, t _{i+1} + \delta _{i+1}) . }$ 

This gives 

$${ \alpha \leq t _1 < {\color{blue}{x _1}} < t _2 < \ldots < t _{n-1} < {\color{blue}{x _{n-1}}} < t _n \leq \beta  }$$ 

with each ${ \lVert f({\color{blue}{x _i}}) - f(t _i) \rVert \leq \varepsilon ({\color{blue}{x _i}} - t _i) }$ and ${ \lVert f(t _{i+1}) - f({\color{blue}{x _i}}) \rVert \leq \varepsilon (t _{i+1} - {\color{blue}{x _i}}) .}$ 

Now each term 

$${ \begin{align*} \lVert f(t _{i+1}) - f(t _i) \rVert \leq &\, \lVert f(t _{i+1}) - f({\color{blue}{x _i}}) \rVert + \lVert f({\color{blue}{x _i}}) - f(t _i)  \rVert \\ \leq &\, \varepsilon (t _{i+1} - {\color{blue}{x _i}}) + \varepsilon ({\color{blue}{x _i}} - t _i) \\ = &\, \varepsilon (t _{i+1} - t _i),   \end{align*} }$$ 

giving 

$${ \begin{align*} &\lVert f(\beta) - f(\alpha) \rVert \\ \leq &\, \lVert f(\beta) - f(t _n) \rVert + \sum _{i=1} ^{n-1} \lVert f(t _{i+1}) - f(t _i) \rVert + \lVert f(t _1) - f(\alpha) \rVert \\ \leq &\, \varepsilon(\beta - t _n) + \sum _{i=1} ^{n-1} \varepsilon (t _{i+1} - t _i) +  \varepsilon (t _1 - \alpha) \\ = &\, \varepsilon (\beta - \alpha).   \end{align*}  }$$ 

As ${ \varepsilon > 0 }$ was arbitrary, ${ f(\beta) = f(\alpha) }$ as needed. ${ \blacksquare }$ 

**Thm** [Integrating maps ${ [a, b] \to L(E, F) }$]:    
Consider reals ${ a < b , }$ and normed spaces ${ E, F }$ with ${ F }$ complete. (So ${ L(E, F) }$ is complete). Consider a continuous map ${ \alpha : [a, b] \to L(E, F) .}$ Now 

$${ \int _a ^b \alpha(t) \, dt  \quad \text{ in } L(E, F)   }$$ 

acts as  

$${ \left( \int _a ^b \alpha (t) \, dt \right) y = \int _a ^b \alpha(t) y   \, dt    }$$ 

for all ${ y \in E . }$    
**Pf**: Fix a ${ y \in E . }$ This gives a continuous linear map 

$${ T : L(E, F) \to F , \quad \lambda \mapsto \lambda (y) . }$$ 

Linearity is clear, and continuity is because 

$${ \sup _{\lambda \neq 0} \frac{\lVert T(\lambda) \rVert}{\lVert \lambda \rVert} = \sup _{\lambda \neq 0} \frac{\lVert \lambda(y) \rVert}{\lVert \lambda \rVert} \leq \lVert y \rVert . }$$ 

We have continuous maps 

$${ [a, b] \overset{\alpha}{\longrightarrow} L(E, F) \overset{T}{\longrightarrow} F  ,   }$$ 

$${ t \longmapsto \alpha(t) \longmapsto \alpha(t) y .}$$ 

We are to show 

$${ \text{To show: } \int _a ^b (T \circ \alpha) (t) \, dt = T \circ \left( \int _a ^b \alpha(t) \, dt   \right) .   }$$ 

There is a sequence of step maps ${ s _n : [a, b] \to L(E, F) }$ with ${ \lVert s _n - \alpha \rVert \to 0 .}$ Now ${ T \circ s _n : [a, b] \to F }$ are also step maps, and 

$${ \begin{align*} \lVert T\circ s _n - T \circ \alpha \rVert = &\, \sup _{t \in [a, b]} \lVert s _n (t) y - \alpha(t) y  \rVert \\ \leq &\, \lVert s _n - \alpha \rVert \lVert y \rVert \to 0 .  \end{align*}  }$$ 

It suffices to show 

$${ \text{Suffices to show: } \int _a ^b (T \circ s _n) (t) \, dt = T \circ \left( \int _a ^b s _n (t) \, dt \right) ,  }$$ 

because then letting ${ n \to \infty }$ gives ${ \int (T \circ \alpha) = T \circ \int \alpha  .}$ 

Say ${ s _n : [a, b] \to L(E, F) }$ is a step map wrt partition ${ \mathcal{P} _n : a = x _0 < \ldots < x _N = b ,}$ and ${ s _n (t) = c _i }$ on each interval ${ t \in (x _{i-1}, x _i) .}$ 

Now ${ T \circ s _n }$ is a step map wrt same partition, and 

$${ \begin{align*} \int _a ^b (T \circ s _n) (t) \, dt = &\sum _{i=1} ^{N} T(c _i) (x _i - x _{i-1}) \\ = &\, \sum _{i=1} ^{N} c _i y \, (x _i - x _{i-1}) \\ = &\, \left( \sum _{i=1} ^{N} c _i (x _i - x _{i-1})  \right) \, y \\ = &\, \left( \int _a ^b s _n (t) \, dt \right) \, y \\ = &\, T \circ \left( \int _a ^b s _n (t) \, dt \right) ,     \end{align*}  }$$ 

as needed. ${ \blacksquare }$ 

**Thm** [Integration by parts]:    
Let ${ E, F, G }$ be complete normed spaces, and 

$${ \bullet : E \times F \to G }$$

a continuous bilinear map.    
Let ${ I \subseteq \mathbb{R} }$ be an open interval, ${ a, b \in I , }$ and 

$${ f : I \to E, \quad g : I \to F  }$$ 

be ${ C ^1 }$ maps. Then 

$${ \begin{align*} &\int _a ^b f(t) \bullet D g (t) \, dt \\ = &\, f(b) \bullet g(b) - f(a) \bullet g(a) - \int _a ^b Df(t) \bullet g(t) \, dt \end{align*} }$$

**Pf**: By product rule, 

$${ D(f \bullet g)(t) = Df(t) \bullet g(t) + f(t) \bullet Dg(t) .  }$$ 

Integrating this gives the required identity.


**Eg**: Consider the map 

$${ A : [0, \pi] \longrightarrow (L(\mathbb{R} ^2, \mathbb{R} ^2), \lVert \ldots \rVert _{\text{op}}) ,    }$$ 

$${ t \longmapsto \begin{pmatrix} \cos(t) &t \\ \sin(t) &t ^2 \end{pmatrix} .  }$$ 

We can study ${ A ^{’} (t) }$ and ${ \int _0 ^\pi A(t) \, dt .}$ 

The map 

$${ A _F  : [0, \pi] \longrightarrow (L(\mathbb{R} ^2, \mathbb{R} ^2), \lVert \ldots \rVert _{F}) \cong (\mathbb{R} ^4, \lVert \cdots \rVert _u)  , }$$ 

$${ t \longmapsto \begin{pmatrix} \cos(t) &t \\ \sin(t) &t ^2 \end{pmatrix} }$$ 

can be readily differentiated and integrated due to the results on component wise differentiation and integration of  maps ${ [a, b] \to \mathbb{R} ^k :}$ 

$${ \begin{align*} &A _F ^{’} (t) = \begin{pmatrix} -\sin(t) &1 \\ \cos(t) &2t \end{pmatrix} \text{ for } t \in (a, b) , \\ &\int _0 ^\pi A _F (t) \, dt =  \begin{pmatrix} 0 &\pi ^2 /2 \\ 2 &\pi ^3 /3  \end{pmatrix} .  \end{align*} }$$ 

But ${ \lVert \cdots \rVert _{\text{op}} }$ and ${ \lVert \cdots \rVert _F }$ are equivalent norms on ${ L(\mathbb{R} ^2, \mathbb{R} ^2) .}$ 

Let ${ t \in (a, b) .}$ As 

$${ \begin{align*} &\frac{\lVert A(t+h) - A(t) - A _F ^{’}(t) h \rVert _{\text{op}} }{\vert h \vert} \\ \leq &\, K \frac{\lVert A(t+h) - A(t) - A _F ^{’}(t) h \rVert _{F} }{\vert h \vert} \to 0  \end{align*}  }$$ 

as ${ h \to 0 , }$ we see derivative 

$${ A ^{’} (t) = A _F ^{’} (t) = \begin{pmatrix} -\sin(t) &1 \\ \cos(t) &2t \end{pmatrix} \text{ for } t \in (a, b)  .}$$ 

There are step maps ${ s _n : [0, \pi] \to (L(\mathbb{R} ^2, \mathbb{R} ^2), \lVert \cdots \rVert _F) }$ with ${  \sup _{t \in [0, \pi]} \lVert s _n (t) - A (t) \rVert _F   \to 0  }$ and 

$${ \left\lVert \int _0 ^\pi s _n (t) \, dt - \int _0 ^\pi A _F (t) \, dt \right\rVert _F \longrightarrow 0 .  }$$ 

Due to equivalence of norms, ${ \sup _{t \in [0, \pi]} \lVert s _n (t) - A (t) \rVert _{\text{op}} \to 0 }$ and 

$${ \left\lVert \int _0 ^\pi s _n (t) \, dt - \int _0 ^\pi A _F (t) \, dt  \right\rVert _{\text{op}}   \to 0 .   }$$ 

So integral 

$${ \int _0 ^{\pi} A(t) \, dt = \int _0 ^{\pi} A _F (t) \, dt = \begin{pmatrix} 0 &\pi ^2 /2 \\ 2 &\pi ^3 /3  \end{pmatrix} .    }$$ 

###### 5. 

$${ \underline{\textbf{Mean value theorem}} }$$ 

**Def** [${ C ^1 }$ maps]: Let ${ E, F }$ be complete normed spaces, and ${ f : U (\subseteq E \text{ open}) \to F .}$    
We say ${ f }$ is ${ C ^1 }$ on ${ U }$ if it is differentiable on ${ U }$ and the derivative 

$${ Df : U \longrightarrow L(E, F)  }$$ 

is continuous. 

**Obs** [${ C ^1 }$ maps ${ \mathbb{R} ^n \to \mathbb{R} ^m }$ and partials]:    
Consider ${ f : U (\subseteq \mathbb{R} ^n \text{ open}) \to \mathbb{R} ^m .}$    
Now ${ f : U \to \mathbb{R} ^m  }$ is ${ C ^1 }$ if and only if all partials ${ D _j f _i : U \to \mathbb{R} }$ exist and are continuous.   

**Pf**: ${ \underline{\Rightarrow} }$ Say ${ f : U \to \mathbb{R} ^m }$ is ${ C ^1 . }$ So ${ Df : U \to L(\mathbb{R} ^n, \mathbb{R} ^m ) }$ exists as a continuous map.    
By previous observation (on differentiating maps ${ \mathbb{R} ^n \to \mathbb{R} ^m }$), for every ${ x \in U }$ all partials ${ D _j f _i (x) }$ exist and ${ Df(x) }$ looks like  

$${ Df(x) = \begin{pmatrix} D _1 f _1 (x) &\cdots &D _n f _1 (x) \\ \vdots &\ddots &\vdots \\ D _1 f _m (x) &\cdots &D _n f _m (x)  \end{pmatrix} .   }$$ 

As ${ U \to (L(\mathbb{R} ^n, \mathbb{R} ^m), \lVert \cdots \rVert _{\text{op}}) ,}$   ${ x \mapsto Df(x) }$ is continuous, so is ${ U \to (L(\mathbb{R} ^n, \mathbb{R} ^m), \lVert \cdots \rVert _F ) \cong (\mathbb{R} ^{mn}, \lVert \cdots \rVert _u)  ,}$ ${ x \mapsto Df(x) .}$    
Hence each component ${ D _j f _i : U \to \mathbb{R} }$ is continuous.     

${ \underline{\Leftarrow} }$ Say all partials ${ D _j f _i : U \to \mathbb{R} }$ exist and are continuous. By previous observation (on differentiating maps ${ \mathbb{R} ^n \to \mathbb{R} ^m }$), for every ${ x \in U , }$ 

$${ \begin{pmatrix} D _1 f _1 (x) &\cdots &D _n f _1 (x) \\ \vdots &\ddots &\vdots \\ D _1 f _m (x) &\cdots &D _n f _m (x)  \end{pmatrix}  }$$ 

works as the derivative of ${ f }$ at ${ x .}$ Continuity of components ${ D _j F _i : U \to \mathbb{R} }$ gives continuity of ${ U \to (L(\mathbb{R} ^n, \mathbb{R} ^m), \lVert \cdots \rVert _F ) , }$ ${ x \mapsto Df(x) .}$ Hence ${ U \to (L(\mathbb{R} ^n, \mathbb{R} ^m), \lVert \cdots \rVert _{\text{op}} ) , }$ ${ x \mapsto Df(x) }$ is continuous, that is ${ f }$ is a ${ C ^1  }$ map.  

**Thm** [Mean value theorem]:    
Let ${ E, F }$ be complete normed spaces, and ${ f : U (\subseteq E \text{ open}) \to F }$ a ${ C ^1 }$ map.     
Consider a segment ${ [[x, y]] = \lbrace x + t(y-x) : t \in [0, 1] \rbrace }$ contained in ${ U .}$ Then

$${ \begin{align*} f(y) - f(x) = &\int _0 ^1 Df(x+t(y-x)) (y-x) \, dt \\ = &\left( \int _0 ^1 Df(x+t(y-x)) \, dt \right) \cdot (y-x) . \end{align*} }$$ 

> Especially 
> 
> $${ \begin{align*} \lVert f(y) - f(x) \rVert \leq &\sup _{t \in [0, 1]} \lVert Df(x + t(y-x)) \rVert \lVert y - x \rVert \\ = &\sup _{v \in [[x, y]]} \lVert Df(v) \rVert \lVert y - x \rVert .  \end{align*} }$$
> 
> As ${ t \mapsto \lVert Df(x + t(y-x)) \rVert }$ is continuous on the compact set ${ [0, 1] , }$ the term 
>
> $${ \sup _{t \in [0, 1]} \lVert Df(x + t(y-x)) \rVert < \infty .}$$ 

**Pf**: Consider

$${ g : [0, 1] \to F, \quad g(t) = f(x + t(y-x)).  }$$

As ${ g ^{’} (t) =  Df(x+t(y-x)) \circ (y-x)  }$ is continuous, 

$${ g(1) - g(0) = \int _0 ^1 g ^{’}(t) \, dt  }$$ 

that is 

$${ f(y) - f(x) = \int _0 ^1 Df(x+t(y-x)) (y-x) \, dt, }$$ 

as needed. 


